Update Finite_Extensions.thy with lots of new results

Finite_Extensions.thy
@@ -17,13 +17,16 @@ definition (in ring) transcendental :: "'a set \<Rightarrow> 'a \<Rightarrow> bo
 abbreviation (in ring) algebraic :: "'a set \<Rightarrow> 'a \<Rightarrow> bool"
   where "algebraic K x \<equiv> \<not> transcendental K x"
 
+definition (in ring) algebraic_set :: "'a set \<Rightarrow> 'a set \<Rightarrow> bool"
+  where "algebraic_set K A \<longleftrightarrow> (\<forall>x \<in> A. (algebraic over K) x)"
+
 definition (in ring) Irr :: "'a set \<Rightarrow> 'a \<Rightarrow> 'a list"
   where "Irr K x = (THE p. p \<in> carrier (K[X]) \<and> pirreducible K p \<and> eval p x = \<zero> \<and> lead_coeff p = \<one>)"
 
 inductive_set (in ring) simple_extension :: "'a set \<Rightarrow> 'a \<Rightarrow> 'a set"
   for K and x where
-    zero: "\<zero> \<in> simple_extension K x" |
-    lin:  "\<lbrakk> k1 \<in> K; k2 \<in> K \<rbrakk> \<Longrightarrow> (k1 \<otimes> x) \<oplus> k2 \<in> simple_extension K x"
+    zero [simp, intro]: "\<zero> \<in> simple_extension K x" |
+    lin:  "\<lbrakk> k1 \<in> simple_extension K x; k2 \<in> K \<rbrakk> \<Longrightarrow> (k1 \<otimes> x) \<oplus> k2 \<in> simple_extension K x"
 
 fun (in ring) finite_extension :: "'a set \<Rightarrow> 'a list \<Rightarrow> 'a set"
   where "finite_extension K xs = foldr (\<lambda>x K'. simple_extension K' x) xs K"
@@ -59,19 +62,443 @@ lemma (in domain) algebraic_imp_non_trivial_ker:
   shows "(algebraic over K) x \<Longrightarrow> a_kernel (K[X]) R (\<lambda>p. eval p x) \<noteq> { [] }"
   using trivial_ker_imp_transcendental[OF assms] unfolding over_def by auto
 
+lemma (in domain) algebraicE:
+  assumes "subring K R" and "x \<in> carrier R" "(algebraic over K) x"
+  obtains p where "p \<in> carrier (K[X])" "p \<noteq> []" "eval p x = \<zero>"
+proof -
+  have "[] \<in> a_kernel (K[X]) R (\<lambda>p. eval p x)"
+    unfolding a_kernel_def' univ_poly_def by auto
+  then obtain p where "p \<in> carrier (K[X])" "p \<noteq> []" "eval p x = \<zero>"
+    using algebraic_imp_non_trivial_ker[OF assms] unfolding a_kernel_def' by blast
+  thus thesis using that by auto
+qed
+
+lemma (in ring) algebraicI:
+  assumes "p \<in> carrier (K[X])" "p \<noteq> []" and "eval p x = \<zero>" shows "(algebraic over K) x"
+  using assms non_trivial_ker_imp_algebraic unfolding a_kernel_def' by auto
+
+lemma (in ring) transcendental_mono:
+  assumes "K \<subseteq> K'" "(transcendental over K') x" shows "(transcendental over K) x"
+proof -
+  have "carrier (K[X]) \<subseteq> carrier (K'[X])"
+    using assms(1) unfolding univ_poly_def polynomial_def by auto
+  thus ?thesis
+    using assms unfolding over_def transcendental_def by (metis inj_on_subset)
+qed
+
+corollary (in ring) algebraic_mono:
+  assumes "K \<subseteq> K'" "(algebraic over K) x" shows "(algebraic over K') x"
+  using transcendental_mono[OF assms(1)] assms(2) unfolding over_def by blast 
+
 lemma (in domain) zero_is_algebraic:
   assumes "subring K R" shows "(algebraic over K) \<zero>"
-proof -
-  have non_trivial_eval: "[ \<one>, \<zero> ] \<in> carrier (K[X])" "eval [ \<one>, \<zero> ] \<zero> = \<zero>"
-    by (auto simp add: univ_poly_def polynomial_def subringE(2-3)[OF assms])
-  show ?thesis
-    using eval_transcendental[OF _ non_trivial_eval] unfolding over_def by auto
+  using algebraicI[OF var_closed(1)[OF assms]] unfolding var_def by auto
+
+lemma (in domain) algebraic_self:
+  assumes "subring K R" and "k \<in> K" shows "(algebraic over K) k"
+proof (rule algebraicI[of "[ \<one>, \<ominus> k ]"])
+  show "[ \<one>, \<ominus> k ] \<in> carrier (K [X])" and "[ \<one>, \<ominus> k ] \<noteq> []"
+    using subringE(2-3,5)[OF assms(1)] assms(2) unfolding univ_poly_def polynomial_def by auto
+  have "k \<in> carrier R"
+    using subringE(1)[OF assms(1)] assms(2) by auto
+  thus "eval [ \<one>, \<ominus> k ] k = \<zero>"
+    by (auto, algebra)
 qed
 
 lemma (in domain) ker_diff_carrier:
-  assumes "subring K R" and "x \<in> carrier R"
+  assumes "subring K R"
   shows "a_kernel (K[X]) R (\<lambda>p. eval p x) \<noteq> carrier (K[X])"
-proof (rule ccontr)
+proof -
+  have "eval [ \<one> ] x \<noteq> \<zero>" and "[ \<one> ] \<in> carrier (K[X])"
+    using subringE(3)[OF assms] unfolding univ_poly_def polynomial_def by auto
+  thus ?thesis
+    unfolding a_kernel_def' by blast
+qed
+
+
+subsection \<open>Minimal Polynomial\<close>
+
+lemma (in domain) minimal_polynomial_is_unique:
+  assumes "subfield K R" and "x \<in> carrier R" "(algebraic over K) x"
+  shows "\<exists>!p \<in> carrier (K[X]). pirreducible K p \<and> eval p x = \<zero> \<and> lead_coeff p = \<one>"
+    (is "\<exists>!p. ?minimal_poly p")
+proof -
+  interpret UP: principal_domain "K[X]"
+    using univ_poly_is_principal[OF assms(1)] .
+
+  let ?ker_gen = "\<lambda>p. p \<in> carrier (K[X]) \<and> pirreducible K p \<and> lead_coeff p = \<one> \<and>
+                    a_kernel (K[X]) R (\<lambda>p. eval p x) = PIdl\<^bsub>K[X]\<^esub> p"
+
+  obtain p where p: "?ker_gen p" and unique: "\<And>q. ?ker_gen q \<Longrightarrow> q = p"
+    using exists_unique_pirreducible_gen[OF assms(1) eval_ring_hom[OF _ assms(2)]
+          algebraic_imp_non_trivial_ker[OF _ assms(2-3)]
+          ker_diff_carrier] subfieldE(1)[OF assms(1)] by auto
+  hence "?minimal_poly p"
+    using UP.cgenideal_self p unfolding a_kernel_def' by auto
+  moreover have "\<And>q. ?minimal_poly q \<Longrightarrow> q = p"
+  proof -
+    fix q assume q: "?minimal_poly q"
+    then have "q \<in> PIdl\<^bsub>K[X]\<^esub> p"
+      using p unfolding a_kernel_def' by auto
+    hence "p \<sim>\<^bsub>K[X]\<^esub> q"
+      using cgenideal_pirreducible[OF assms(1)] p q by simp
+    hence "a_kernel (K[X]) R (\<lambda>p. eval p x) = PIdl\<^bsub>K[X]\<^esub> q"
+      using UP.associated_iff_same_ideal q p by simp
+    thus "q = p"
+      using unique q by simp
+  qed
+  ultimately show ?thesis by blast
+qed
+
+lemma (in domain) IrrE:
+  assumes "subfield K R" and "x \<in> carrier R" "(algebraic over K) x"
+  shows "Irr K x \<in> carrier (K[X])" and "pirreducible K (Irr K x)"
+    and "lead_coeff (Irr K x) = \<one>" and "eval (Irr K x) x = \<zero>"
+  using theI'[OF minimal_polynomial_is_unique[OF assms]] unfolding Irr_def by auto
+
+lemma (in domain) Irr_generates_ker:
+  assumes "subfield K R" and "x \<in> carrier R" "(algebraic over K) x"
+  shows "a_kernel (K[X]) R (\<lambda>p. eval p x) = PIdl\<^bsub>K[X]\<^esub> (Irr K x)"
+proof -
+  obtain q
+    where q: "q \<in> carrier (K[X])" "pirreducible K q"
+      and ker: "a_kernel (K[X]) R (\<lambda>p. eval p x) = PIdl\<^bsub>K[X]\<^esub> q"
+    using exists_unique_pirreducible_gen[OF assms(1) eval_ring_hom[OF _ assms(2)]
+          algebraic_imp_non_trivial_ker[OF _ assms(2-3)]
+          ker_diff_carrier] subfieldE(1)[OF assms(1)] by auto
+  have "Irr K x \<in> PIdl\<^bsub>K[X]\<^esub> q"
+    using IrrE(1,4)[OF assms] ker unfolding a_kernel_def' by auto
+  thus ?thesis
+    using cgenideal_pirreducible[OF assms(1) q(1-2) IrrE(2)[OF assms]] q(1) IrrE(1)[OF assms]
+          cring.associated_iff_same_ideal[OF univ_poly_is_cring[OF subfieldE(1)[OF assms(1)]]]
+    unfolding ker
+    by simp
+qed
+
+lemma (in domain) Irr_minimal:
+  assumes "subfield K R" and "x \<in> carrier R" "(algebraic over K) x"
+    and "p \<in> carrier (K[X])" "eval p x = \<zero>" shows "(Irr K x) pdivides p"
+proof -
+  interpret UP: principal_domain "K[X]"
+    using univ_poly_is_principal[OF assms(1)] .
+
+  have "p \<in> PIdl\<^bsub>K[X]\<^esub> (Irr K x)"
+    using Irr_generates_ker[OF assms(1-3)] assms(4-5) unfolding a_kernel_def' by auto
+  hence "(Irr K x) divides\<^bsub>K[X]\<^esub> p"
+    using UP.to_contain_is_to_divide IrrE(1)[OF assms(1-3)]
+    by (meson UP.cgenideal_ideal UP.cgenideal_minimal assms(4))
+  thus ?thesis
+    unfolding pdivides_iff_shell[OF assms(1) IrrE(1)[OF assms(1-3)] assms(4)] .
+qed
+
+lemma (in domain) rupture_of_Irr:
+  assumes "subfield K R" and "x \<in> carrier R" "(algebraic over K) x" shows "field (Rupt K (Irr K x))"
+  using rupture_is_field_iff_pirreducible[OF assms(1)] IrrE(1-2)[OF assms] by simp
+
+
+subsection \<open>Simple Extensions\<close>
+
+lemma (in ring) simple_extension_consistent:
+  assumes "subring K R" shows "ring.simple_extension (R \<lparr> carrier := K \<rparr>) = simple_extension"
+proof -
+  interpret K: ring "R \<lparr> carrier := K \<rparr>"
+    using subring_is_ring[OF assms] .
+
+  have "\<And>K' x. K.simple_extension  K' x \<subseteq> simple_extension K' x"
+  proof
+    fix K' x a show "a \<in> K.simple_extension  K' x \<Longrightarrow> a \<in> simple_extension K' x"
+      by (induction rule: K.simple_extension.induct) (auto simp add: simple_extension.lin)
+  qed
+  moreover
+  have "\<And>K' x. simple_extension K' x \<subseteq> K.simple_extension  K' x"
+  proof
+    fix K' x a assume a: "a \<in> simple_extension K' x" thus "a \<in> K.simple_extension  K' x"
+      using K.simple_extension.zero K.simple_extension.lin
+      by (induction rule: simple_extension.induct) (simp)+
+  qed
+  ultimately show ?thesis by blast
+qed
+
+lemma (in ring) mono_simple_extension:
+  assumes "K \<subseteq> K'" shows "simple_extension K x \<subseteq> simple_extension K' x"
+proof
+  fix a assume "a \<in> simple_extension K x" thus "a \<in> simple_extension K' x"
+  proof (induct a rule: simple_extension.induct, simp)
+    case lin thus ?case using simple_extension.lin assms by blast
+  qed
+qed
+
+lemma (in ring) simple_extension_incl:
+  assumes "K \<subseteq> carrier R" and "x \<in> carrier R" shows "K \<subseteq> simple_extension K x"
+proof
+  fix k assume "k \<in> K" thus "k \<in> simple_extension K x"
+    using simple_extension.lin[OF simple_extension.zero, of k K x] assms by auto
+qed
+
+lemma (in ring) simple_extension_mem:
+  assumes "subring K R" and "x \<in> carrier R" shows "x \<in> simple_extension K x"
+proof -
+  have "\<one> \<in> simple_extension K x"
+    using simple_extension_incl[OF _ assms(2)] subringE(1,3)[OF assms(1)] by auto
+  thus ?thesis
+    using simple_extension.lin[OF _ subringE(2)[OF assms(1)], of \<one> x] assms(2) by auto
+qed
+
+lemma (in ring) simple_extension_carrier:
+  assumes "x \<in> carrier R" shows "simple_extension (carrier R) x = carrier R"
+proof
+  show "carrier R \<subseteq> simple_extension (carrier R) x"
+    using simple_extension_incl[OF _ assms] by auto
+next
+  show "simple_extension (carrier R) x \<subseteq> carrier R"
+  proof
+    fix a assume "a \<in> simple_extension (carrier R) x" thus "a \<in> carrier R"
+      by (induct a rule: simple_extension.induct) (auto simp add: assms)
+  qed
+qed
+
+lemma (in ring) simple_extension_in_carrier:
+  assumes "K \<subseteq> carrier R" and "x \<in> carrier R" shows "simple_extension K x \<subseteq> carrier R"
+  using mono_simple_extension[OF assms(1)] simple_extension_carrier[OF assms(2)] by auto
+
+lemma (in ring) simple_extension_subring_incl:
+  assumes "subring K' R" and "K \<subseteq> K'" "x \<in> K'" shows "simple_extension K x \<subseteq> K'"
+  using ring.simple_extension_in_carrier[OF subring_is_ring[OF assms(1)]] assms(2-3)
+  unfolding simple_extension_consistent[OF assms(1)] by simp
+
+lemma (in ring) simple_extension_as_eval_img:
+  assumes "K \<subseteq> carrier R" "x \<in> carrier R"
+  shows "simple_extension K x = (\<lambda>p. eval p x) ` carrier (K[X])"
+proof
+  show "simple_extension K x \<subseteq> (\<lambda>p. eval p x) ` carrier (K[X])"
+  proof
+    fix a assume "a \<in> simple_extension K x" thus "a \<in> (\<lambda>p. eval p x) ` carrier (K[X])"
+    proof (induction rule: simple_extension.induct)
+      case zero
+      have "polynomial K []" and "eval [] x = \<zero>"
+        unfolding polynomial_def by simp+
+      thus ?case
+        unfolding univ_poly_carrier by force
+    next
+      case (lin k1 k2)
+      then obtain p where p: "p \<in> carrier (K[X])" "polynomial K p" "eval p x = k1"
+        by (auto simp add: univ_poly_carrier)
+      hence "set p \<subseteq> carrier R" and "k2 \<in> carrier R"
+        using assms(1) lin(2) unfolding polynomial_def by auto
+      hence "eval (normalize (p @ [ k2 ])) x = k1 \<otimes> x \<oplus> k2"
+        using eval_append_aux[of p k2 x] eval_normalize[of "p @ [ k2 ]" x] assms(2) p(3) by auto
+      thus ?case
+        using normalize_gives_polynomial[of "p @ [ k2 ]"] polynomial_incl[OF p(2)] lin(2)
+        unfolding univ_poly_carrier by force
+    qed
+  qed
+next
+  show "(\<lambda>p. eval p x) ` carrier (K[X]) \<subseteq> simple_extension K x"
+  proof
+    fix a assume "a \<in> (\<lambda>p. eval p x) ` carrier (K[X])"
+    then obtain p where p: "set p \<subseteq> K" "eval p x = a"
+      using polynomial_incl unfolding univ_poly_def by auto
+    thus "a \<in> simple_extension K x"
+    proof (induct "length p" arbitrary: p a)
+      case 0 thus ?case
+        using simple_extension.zero by simp
+    next
+      case (Suc n)
+      obtain p' k where p: "p = p' @ [ k ]"
+        using Suc(2) by (metis list.size(3) nat.simps(3) rev_exhaust)
+      hence "a = (eval p' x) \<otimes> x \<oplus> k"
+        using eval_append_aux[of p' k x] Suc(3-4) assms unfolding p by auto
+      moreover have "eval p' x \<in> simple_extension K x"
+        using Suc(1-3) unfolding p by auto
+      ultimately show ?case
+        using simple_extension.lin Suc(3) unfolding p by auto
+    qed
+  qed
+qed
+
+corollary (in domain) simple_extension_is_subring:
+  assumes "subring K R" "x \<in> carrier R" shows "subring (simple_extension K x) R"
+  using ring_hom_ring.img_is_subring[OF eval_ring_hom[OF assms]
+        ring.carrier_is_subring[OF univ_poly_is_ring[OF assms(1)]]]
+        simple_extension_as_eval_img[OF subringE(1)[OF assms(1)] assms(2)]
+  by simp
+
+corollary (in domain) simple_extension_minimal:
+  assumes "subring K R" "x \<in> carrier R"
+  shows "simple_extension K x = \<Inter> { K'. subring K' R \<and> K \<subseteq> K' \<and> x \<in> K' }"
+  using simple_extension_is_subring[OF assms] simple_extension_mem[OF assms]
+        simple_extension_incl[OF subringE(1)[OF assms(1)] assms(2)] simple_extension_subring_incl
+  by blast
+
+corollary (in domain) simple_extension_isomorphism:
+  assumes "subring K R" "x \<in> carrier R"
+  shows "(K[X]) Quot (a_kernel (K[X]) R (\<lambda>p. eval p x)) \<simeq> R \<lparr> carrier := simple_extension K x \<rparr>"
+  using ring_hom_ring.FactRing_iso_set_aux[OF eval_ring_hom[OF assms]]
+        simple_extension_as_eval_img[OF subringE(1)[OF assms(1)] assms(2)]
+  unfolding is_ring_iso_def by auto
+
+corollary (in domain) simple_extension_of_algebraic:
+  assumes "subfield K R" and "x \<in> carrier R" "(algebraic over K) x"
+  shows "Rupt K (Irr K x) \<simeq> R \<lparr> carrier := simple_extension K x \<rparr>"
+  using simple_extension_isomorphism[OF subfieldE(1)[OF assms(1)] assms(2)]
+  unfolding Irr_generates_ker[OF assms] rupture_def by simp
+
+corollary (in domain) simple_extension_of_transcendental:
+  assumes "subring K R" and "x \<in> carrier R" "(transcendental over K) x"
+  shows "K[X] \<simeq> R \<lparr> carrier := simple_extension K x \<rparr>"
+  using simple_extension_isomorphism[OF _ assms(2), of K] assms(1)
+        ring_iso_trans[OF ring.FactRing_zeroideal(2)[OF univ_poly_is_ring]]
+  unfolding transcendental_imp_trivial_ker[OF assms(3)] univ_poly_zero
+  by auto
+
+proposition (in domain) simple_extension_subfield_imp_algebraic:
+  assumes "subring K R" "x \<in> carrier R"
+  shows "subfield (simple_extension K x) R \<Longrightarrow> (algebraic over K) x"
+proof -
+  assume simple_ext: "subfield (simple_extension K x) R" show "(algebraic over K) x"
+  proof (rule ccontr)
+    assume "\<not> (algebraic over K) x" then have "(transcendental over K) x"
+      unfolding over_def by simp
+    then obtain h where h: "h \<in> ring_iso (R \<lparr> carrier := simple_extension K x \<rparr>) (K[X])"
+      using ring_iso_sym[OF univ_poly_is_ring simple_extension_of_transcendental] assms
+      unfolding is_ring_iso_def by blast
+    then interpret Hom: ring_hom_ring "R \<lparr> carrier := simple_extension K x \<rparr>" "K[X]" h
+      using subring_is_ring[OF simple_extension_is_subring[OF assms]]
+            univ_poly_is_ring[OF assms(1)] assms h
+      by (auto simp add: ring_hom_ring_def ring_hom_ring_axioms_def ring_iso_def)
+    have "field (K[X])"
+      using field.ring_iso_imp_img_field[OF subfield_iff(2)[OF simple_ext] h]
+      unfolding Hom.hom_one Hom.hom_zero by simp
+    moreover have "\<not> field (K[X])"
+      using univ_poly_not_field[OF assms(1)] .
+    ultimately show False by simp
+  qed
+qed
+
+proposition (in domain) simple_extension_is_subfield:
+  assumes "subfield K R" "x \<in> carrier R"
+  shows "subfield (simple_extension K x) R \<longleftrightarrow> (algebraic over K) x"
+proof
+  assume alg: "(algebraic over K) x"
+  then obtain h where h: "h \<in> ring_iso (Rupt K (Irr K x)) (R \<lparr> carrier := simple_extension K x \<rparr>)"
+    using simple_extension_of_algebraic[OF assms] unfolding is_ring_iso_def by blast
+  have rupt_field: "field (Rupt K (Irr K x))" and "ring (R \<lparr> carrier := simple_extension K x \<rparr>)"
+    using subring_is_ring[OF simple_extension_is_subring[OF subfieldE(1)]]
+          rupture_of_Irr[OF assms alg] assms by simp+
+  then interpret Hom: ring_hom_ring "Rupt K (Irr K x)" "R \<lparr> carrier := simple_extension K x \<rparr>" h
+    using h cring.axioms(1)[OF domain.axioms(1)[OF field.axioms(1)]]
+    by (auto simp add: ring_hom_ring_def ring_hom_ring_axioms_def ring_iso_def)
+  show "subfield (simple_extension K x) R"
+    using field.ring_iso_imp_img_field[OF rupt_field h] subfield_iff(1)[OF _
+          simple_extension_in_carrier[OF subfieldE(3)[OF assms(1)] assms(2)]]
+    by simp
+next
+  assume simple_ext: "subfield (simple_extension K x) R" thus "(algebraic over K) x"
+    using simple_extension_subfield_imp_algebraic[OF subfieldE(1)[OF assms(1)] assms(2)] by simp
+qed
+
+(*
+corollary (in domain)
+  assumes "subfield K R" "x \<in> carrier R"
+  shows "dimension (degree (Irr K x)) K (simple_extension K x) \<longleftrightarrow> (algebraic over K) x"
+  sorry
+*)
+
+
+subsection \<open>Finite Extensions\<close>
+
+lemma (in ring) finite_extension_consistent:
+  assumes "subring K R" shows "ring.finite_extension (R \<lparr> carrier := K \<rparr>) = finite_extension"
+proof -
+  have "\<And>K' xs. ring.finite_extension (R \<lparr> carrier := K \<rparr>) K' xs = finite_extension K' xs"
+  proof -
+    fix K' xs show "ring.finite_extension (R \<lparr> carrier := K \<rparr>) K' xs = finite_extension K' xs"
+      using ring.finite_extension.simps[OF subring_is_ring[OF assms]]
+            simple_extension_consistent[OF assms] by (induct xs) (auto)
+  qed
+  thus ?thesis by blast
+qed
+
+lemma (in ring) mono_finite_extension:
+  assumes "K \<subseteq> K'" shows "finite_extension K xs \<subseteq> finite_extension K' xs"
+  using mono_simple_extension assms by (induct xs) (auto)
+
+lemma (in ring) finite_extension_carrier:
+  assumes "set xs \<subseteq> carrier R" shows "finite_extension (carrier R) xs = carrier R"
+  using assms simple_extension_carrier by (induct xs) (auto)
+
+lemma (in ring) finite_extension_in_carrier:
+  assumes "K \<subseteq> carrier R" and "set xs \<subseteq> carrier R" shows "finite_extension K xs \<subseteq> carrier R"
+  using assms simple_extension_in_carrier by (induct xs) (auto)
+
+lemma (in ring) finite_extension_subring_incl:
+  assumes "subring K' R" and "K \<subseteq> K'" "set xs \<subseteq> K'" shows "finite_extension K xs \<subseteq> K'"
+  using ring.finite_extension_in_carrier[OF subring_is_ring[OF assms(1)]] assms(2-3)
+  unfolding finite_extension_consistent[OF assms(1)] by simp
+
+lemma (in ring) finite_extension_incl_aux:
+  assumes "K \<subseteq> carrier R" and "x \<in> carrier R" "set xs \<subseteq> carrier R"
+  shows "finite_extension K xs \<subseteq> finite_extension K (x # xs)"
+  using simple_extension_incl[OF finite_extension_in_carrier[OF assms(1,3)] assms(2)] by simp
+
+lemma (in ring) finite_extension_incl:
+  assumes "K \<subseteq> carrier R" and "set xs \<subseteq> carrier R" shows "K \<subseteq> finite_extension K xs"
+  using finite_extension_incl_aux[OF assms(1)] assms(2) by (induct xs) (auto)
+
+lemma (in ring) finite_extension_as_eval_img:
+  assumes "K \<subseteq> carrier R" and "x \<in> carrier R" "set xs \<subseteq> carrier R"
+  shows "finite_extension K (x # xs) = (\<lambda>p. eval p x) ` carrier ((finite_extension K xs) [X])"
+  using simple_extension_as_eval_img[OF finite_extension_in_carrier[OF assms(1,3)] assms(2)] by simp
+
+lemma (in domain) finite_extension_is_subring:
+  assumes "subring K R" "set xs \<subseteq> carrier R" shows "subring (finite_extension K xs) R"
+  using assms simple_extension_is_subring by (induct xs) (auto)
+
+corollary (in domain) finite_extension_mem:
+  assumes "subring K R" "set xs \<subseteq> carrier R" shows "set xs \<subseteq> finite_extension K xs"
+proof -
+  { fix x xs assume "x \<in> carrier R" "set xs \<subseteq> carrier R"
+    hence "x \<in> finite_extension K (x # xs)"
+      using simple_extension_mem[OF finite_extension_is_subring[OF assms(1), of xs]] by simp }
+  note aux_lemma = this
+  show ?thesis
+    using aux_lemma finite_extension_incl_aux[OF subringE(1)[OF assms(1)]] assms(2)
+    by (induct xs) (simp, smt insert_subset list.simps(15) subset_trans) 
+qed
+
+corollary (in domain) finite_extension_minimal:
+  assumes "subring K R" "set xs \<subseteq> carrier R"
+  shows "finite_extension K xs = \<Inter> { K'. subring K' R \<and> K \<subseteq> K' \<and> set xs \<subseteq> K' }"
+  using finite_extension_is_subring[OF assms] finite_extension_mem[OF assms]
+        finite_extension_incl[OF subringE(1)[OF assms(1)] assms(2)] finite_extension_subring_incl
+  by blast
+
+corollary (in domain) finite_extension_same_set:
+  assumes "subring K R" "set xs \<subseteq> carrier R" "set xs = set ys"
+  shows "finite_extension K xs = finite_extension K ys"
+  using finite_extension_minimal[OF assms(1)] assms(2-3) by auto
+
+proposition (in domain) finite_extension_is_subfield:
+  assumes "subfield K R" "set xs \<subseteq> carrier R"
+  shows "subfield (finite_extension K xs) R \<longleftrightarrow> (algebraic_set over K) (set xs)"
+proof
+  have "(\<And>x. x \<in> set xs \<Longrightarrow> (algebraic over K) x) \<Longrightarrow> subfield (finite_extension K xs) R"
+    using simple_extension_is_subfield algebraic_mono assms
+    by (induct xs) (auto, metis finite_extension.simps finite_extension_incl subring_props(1))
+  thus "(algebraic_set over K) (set xs) \<Longrightarrow> subfield (finite_extension K xs) R"
+    unfolding algebraic_set_def over_def by auto
+next
+(*
+  { fix x xs
+    assume x: "x \<in> carrier R" and xs: "set xs \<subseteq> carrier R"
+      and field: "subfield (finite_extension K (x # xs)) R"
+    hence "(algebraic over K) x"
+*)
+
+  assume "subfield (finite_extension K xs) R" show "(algebraic_set over K) (set xs)"
+    sorry
+qed
+
 
 (*
 lemma (in ring) transcendental_imp_trivial_ker:
@@ -119,45 +546,7 @@ lemma (in domain) algebraic_iff:
   using non_trivial_ker_imp_algebraic[OF assms(2)] algebraic_imp_non_trivial_ker[OF assms] by auto
 *)
 
-(*
-proof -
-  define P :: "'a list \<Rightarrow> bool"
-    where "P = (\<lambda>p. p \<noteq> [] \<and> pirreducible K p \<and>
-                    set p \<subseteq> K \<and> eval p x = \<zero> \<and> lead_coeff p = \<one>)"
 
-  obtain q
-    where "polynomial (R \<lparr> carrier := K \<rparr>) q"
-    and "pirreducible K q"
-    and "a_kernel (univ_poly (R \<lparr> carrier := K \<rparr>)) (R \<lparr> carrier := K \<rparr>) (\<lambda>p. eval p x) =
-         PIdl\<^bsub>(univ_poly (R \<lparr> carrier := K \<rparr>))\<^esub> q"
-    using field.exists_ker_generator_pirreducible[OF subfield_iff(2)[OF assms(1)]]
-
-  hence "Irr K x = (THE p. P p)"
-    unfolding Irr_def P_def by auto
-  moreover have p: "P p" sorry
-  moreover have "\<And>q. P q \<Longrightarrow> p = q" sorry
-*)
-(*
-  ultimately have "Irr K x = p"
-    by (metis the_equality)
-  thus "Irr K x \<noteq> []"
-    and "pirreducible (R \<lparr> carrier := K \<rparr>) (Irr K x)"
-    and "set (Irr K x) \<subseteq> K"
-    and "eval (Irr K x) x = \<zero>"
-    and "lead_coeff (Irr K x) = \<one>"
-    using p unfolding P_def by auto
-*)
-
-
-(*
-lemma (in domain) Irr_exists:
-  assumes "subring K R" "x \<in> carrier R"
-*)
-
-lemma (in domain) Irr_is_polynomial:
-  assumes "subring K R" "x \<in> carrier R"
-  shows "polynomial R (Irr K x)"
-  sorry
 (*
 lemma (in field)
   assumes "subfield K R"
